proofs/zero_coupon_bond.v
@@ -28,50 +28,36 @@ Proof.
   destruct_join H1.
   - insert_consistent s Ss.
     induction St; subst s'.
-    -- inversion_event Ev. find_contradiction M.
-    -- ctr_case_analysis ctr ctr0.
-       execute_own ctr H9.
-       case_analysis H9.
-       case_analysis H12.
-       ++ eexists. split.
-          +++ eapply steps_does_not_remove_transactions; eauto.
-              simpl. subst ledger'. right. left. eauto.
-          +++ repeat split; trivial. resolve_owner H4.
-       ++ eexists. split.
-          +++ eapply steps_does_not_remove_transactions; eauto.
-              simpl. subst ledger'. left. eauto.
-          +++ repeat split; trivial. resolve_owner H4.
-    -- not_or ctr ctr0 H6.
-    -- not_or ctr ctr0 H6.
-    -- ctr_case_analysis ctr ctr0. inversion_event Ev. find_contradiction M.
-    -- find_contradiction M.
+    + inversion_event Ev. find_contradiction M.
+    + ctr_case_analysis ctr ctr0.
+      execute_own ctr H9.
+      case_analysis H9.
+      case_analysis H12.
+      * eexists. split.
+        ** eapply steps_does_not_remove_transactions; eauto.
+           simpl. subst ledger'. right. left. eauto.
+        ** repeat split; trivial. resolve_owner H4.
+      * eexists. split.
+        ** eapply steps_does_not_remove_transactions; eauto.
+           simpl. subst ledger'. left. eauto.
+        ** repeat split; trivial. resolve_owner H4.
+    + not_or ctr ctr0 H6.
+    + not_or ctr ctr0 H6.
+    + ctr_case_analysis ctr ctr0. inversion_event Ev. find_contradiction M.
+    + find_contradiction M.
   - insert_consistent s Ss.
     induction St; subst s'.
-    -- inversion_event Ev. find_contradiction_del M.
-    -- ctr_case_analysis ctr ctr0.
-       subst ctr. inversion_event Ev.
-       simpl in *.
-       execute_own ctr H9.
-       case_analysis H9.
-       case_analysis H12.
-       ++ eexists. split.
-          +++ eapply steps_does_not_remove_transactions; eauto.
-              simpl. subst ledger'. right. left. eauto.
-          +++ repeat split; trivial. resolve_owner H4.
-       ++ eexists. split.
-          +++ eapply steps_does_not_remove_transactions; eauto.
-              simpl. subst ledger'. left. eauto.
-          +++ repeat split; trivial. resolve_owner H4.
-    -- not_or ctr ctr0 H6.
-    -- not_or ctr ctr0 H6.
-    -- ctr_case_analysis ctr ctr0. inversion_event Ev. find_contradiction M.
-    -- find_contradiction M.
-
-    insert_consistent s Ss.
-
-
-    insert_consistent s' St.
-    find_contradiction_del M.
+    + inversion_event Ev. find_contradiction_del M.
+    + ctr_case_analysis ctr ctr0.
+      inversion_event Ev. find_contradiction_del M.
+    + not_or ctr ctr0 H6.
+    + not_or ctr ctr0 H6.
+    + ctr_case_analysis ctr ctr0.
+      execute_own ctr H7.
+      case_analysis H7; simpl in *; rewrite <- T in *.
+      * eapply ltb_sound_true in H0. contradict H0. omega.
+      * case_analysis H10.
+    + find_contradiction_del M.
 Qed.
 
 Print zcb_O_to_I.
@@ -95,29 +81,42 @@ Lemma inner_ctr_proof:
 Proof.
   intros.
   destruct_join H1.
-  insert_consistent s Ss.
-  induction St; subst s'.
-  - inversion_event Ev. find_contradiction M.
-  - ctr_case_analysis ctr ctr0.
-    execute_own ctr H10.
-    case_if H10.
-    case_if H14.
-    + eexists. split.
-      ++ eapply steps_does_not_remove_transactions; eauto.
-         subst ledger'. simpl. left. eauto.
-      ++ repeat split; trivial. resolve_owner H5.
-    + eapply ltb_sound_false in H10. contradict H10. rewrite <- T. unfold Δ. omega.
-  - not_or ctr ctr0 H7.
-  - not_or ctr ctr0 H7.
-  - ctr_case_analysis ctr ctr0. inversion_event Ev. find_contradiction M.
-  - find_contradiction M.
+  - insert_consistent s Ss.
+    induction St; subst s'.
+    + inversion_event Ev. find_contradiction M.
+    + ctr_case_analysis ctr ctr0.
+      execute_own ctr H10.
+      case_if H10.
+      case_if H14.
+      * eexists. split.
+        ** eapply steps_does_not_remove_transactions; eauto.
+           subst ledger'. simpl. left. eauto.
+      ** repeat split; trivial. resolve_owner H5.
+      * eapply ltb_sound_false in H10. contradict H10. rewrite <- T. unfold Δ. omega.
+    + not_or ctr ctr0 H7.
+    + not_or ctr ctr0 H7.
+    + ctr_case_analysis ctr ctr0. inversion_event Ev. find_contradiction M.
+    + find_contradiction M.
+  - insert_consistent s Ss.
+    induction St; subst s'.
+    + inversion_event Ev. find_contradiction_del M.
+    + ctr_case_analysis ctr ctr0.
+       inversion_event Ev. find_contradiction_del M.
+    + not_or ctr ctr0 H7.
+    + not_or ctr ctr0 H7.
+    + ctr_case_analysis ctr ctr0.
+      execute_own ctr H8.
+      case_if H8; simpl in *.
+      * rewrite <- T in H0. apply ltb_sound_true in H0. contradict H0. omega.
+      * case_if H11.
+    + find_contradiction_del M.
 Qed.
 
 Proposition zcb_I_to_O:
-  forall s1 s2 ctr_id dsc_id now period I O sc ctr,
+  forall s1 s2 ctr_id gen_ctr dsc_id now period I O sc ctr,
     consistent_state s1 ->
     ctr = finctr ctr_id dsc_id (zcb_desc now period) I O O sc ->
-    joins_generated O ctr s1 s2 now (now + period) ->
+    joins_generated O ctr gen_ctr s1 s2 now (now + period) ->
     O <> 0 ->
     period > Δ ->
     exists tr,
@@ -128,37 +127,50 @@ Proposition zcb_I_to_O:
 Proof.
   intros.
   destruct_join_gen H1.
-  insert_consistent s Ss.
-  insert_consistent s' St.
-  induction St; subst s'.
-  - inversion_event Ev. find_contradiction M.
-  - ctr_case_analysis ctr ctr1.
-    simpl in Ev. inversion_event Ev.
-    execute_own ctr H11.
-    case_analysis H11.
-    case_analysis H15.
-    + eexists. split.
-      eapply steps_does_not_remove_transactions. exact Ss0.
-      subst ledger'. simpl. left. eauto.
-      repeat split; trivial.
-      simpl. resolve_owner H6.
-    + destruct_join J.
-      simpl in Exec.
-      rewrite H0, H11 in Exec.
-      inversion Exec. clear Exec. subst res.
-      simpl in M0. destruct M0 as [M0 | M0]; try contradiction.
-      eapply inner_ctr_proof; eauto.
-      unfold joins. exists s0, s'. unfold At.
-      repeat split; subst ctr0; simpl in *; try exact M1; trivial.
-  - not_or ctr ctr1 H8.
-  - not_or ctr ctr1 H8.
-  - ctr_case_analysis ctr ctr1. inversion_event Ev. find_contradiction M.
-  - find_contradiction M.
+  - insert_consistent s Ss.
+    insert_consistent s' St.
+    induction St; subst s'.
+    + inversion_event Ev. find_contradiction M.
+    + ctr_case_analysis ctr ctr0.
+      simpl in Ev. inversion_event Ev.
+      execute_own ctr H11.
+      case_analysis H11.
+      case_analysis H15.
+      * eexists. split.
+        eapply steps_does_not_remove_transactions. exact Ss0.
+        subst ledger'. simpl. left. eauto.
+        repeat split; trivial.
+        simpl. resolve_owner H6.
+      * destruct_join J.
+        ** simpl in Exec.
+           rewrite H0, H11 in Exec.
+           inversion Exec. clear Exec. subst res.
+           simpl in M0. destruct M0 as [M0 | M0]; try contradiction.
+           eapply inner_ctr_proof; eauto.
+           unfold joins. exists s0, s'. unfold At.
+           repeat split; simpl in *; auto.
+           left. unfold executed. repeat split; trivial;
+           simpl; subst gen_ctr; try exact M1; simpl; auto.
+        ** simpl in Exec.
+           rewrite H0, H11 in Exec.
+           inversion Exec. clear Exec. subst res.
+           simpl in M0. destruct M0 as [M0 | M0]; try contradiction.
+           eapply inner_ctr_proof; eauto.
+           unfold joins. exists s0, s'. unfold At.
+           repeat split; simpl in *; auto.
+           right. unfold executed. repeat split; trivial;
+           simpl; subst gen_ctr; try exact M1; simpl; auto.
+    + not_or ctr ctr0 H8.
+    + not_or ctr ctr0 H8.
+    + ctr_case_analysis ctr ctr0. inversion_event Ev. find_contradiction M.
+    + find_contradiction M.
 Qed.
 
 Print zcb_I_to_O.
 
 
+(* Fact: if the owner does not join the contract in time, the contract is deleted *)
+(* Lemma: joining an expired contract triggers Delete *)
 Lemma O_joins_generated_too_late_inner:
   forall s1 s2 c_id dsc_id now period I O sc ctr T,
     consistent_state s1 ->
@@ -171,389 +183,55 @@ Lemma O_joins_generated_too_late_inner:
 Proof.
   intros.
   destruct_join H1.
-  insert_consistent s Ss.
-  induction St; subst s'.
-  - inversion_event Ev. find_contradiction M.
-  - ctr_case_analysis ctr ctr0.
-    execute_own ctr H11.
-    simpl in *.
-    case_if H11.
-    case_if H14; rewrite T0 in *; apply ltb_sound_false in H0; contradict H0; omega.
-  - not_or ctr ctr0 H8.
-  - not_or ctr ctr0 H8.
-  - ctr_case_analysis ctr ctr0. inversion_event Ev. find_contradiction M.
-  - find_contradiction M.
+  - insert_consistent s Ss.
+    induction St; subst s'.
+    + inversion_event Ev. find_contradiction M.
+    + ctr_case_analysis ctr ctr0.
+      execute_own ctr H11.
+      simpl in *.
+      case_if H11.
+      case_if H14; rewrite T0 in *; apply ltb_sound_false in H0; contradict H0; omega.
+    + not_or ctr ctr0 H8.
+    + not_or ctr ctr0 H8.
+    + ctr_case_analysis ctr ctr0. inversion_event Ev. find_contradiction M.
+    + find_contradiction M.
+  - eapply steps_does_not_remove_events; eauto.
 Qed.
 
 
-  Lemma O_joins_generated_too_late:
-  forall s1 s2 c_id dsc_id now period I O sc ctr T,
+Proposition O_joins_generated_too_late:
+  forall s1 s2 c_id gen_ctr dsc_id now period I O sc ctr T,
     consistent_state s1 ->
     ctr = finctr c_id dsc_id (zcb_desc now period) I O O sc ->
-    joins_generated O ctr s1 s2 now T ->
+    joins_generated O ctr gen_ctr s1 s2 now T ->
     T > now + period + Δ ->
     period > Δ ->
     O <> 0 ->
-    exists ctr',
-      In (Deleted (ctr_id ctr')) (m_events s2) /\
-      ctr_primitive ctr' = (At (now + period) (Scale 11 (One USD))) /\
-      ctr_issuer ctr = I /\
-      ctr_proposed_owner ctr = O /\
-      ctr_scale ctr = sc.
+    In (Deleted (ctr_id gen_ctr)) (m_events s2).
 Proof.
   intros.
   destruct_join_gen H1.
-  insert_consistent s Ss.
-  induction St; subst s'.
-  - inversion_event Ev. find_contradiction M.
-  - ctr_case_analysis ctr ctr1.
-    execute_own ctr H11.
-    case_analysis H11.
-    case_analysis H14.
-    + rewrite <- T0 in *.
-      apply ltb_sound_true in H11.
-      apply ltb_sound_false in H0.
-      contradict H0. unfold Δ. omega.
-    + destruct_join J. simpl in Exec.
-      rewrite H0, H11 in Exec.
-      inversion Exec. subst res.
-      simpl. eexists.
-      split. eapply steps_does_not_remove_events; eauto.
-      eexists. repeat split; trivial.
-  - not_or ctr ctr1 H7.
-  - not_or ctr ctr1 H7.
-  - ctr_case_analysis ctr ctr1. inversion_event Ev. find_contradiction M.
-  - find_contradiction M.
-Qed.
-
-
-(* 
-Proposition zcb_I_to_O:
-  forall s1 s2 ctr_id dsc_id now period I O sc ctr,
-    consistent_state s1 ->
-    ctr = finctr ctr_id dsc_id (zcb_desc now period) I O O sc ->
-    joins_generated O ctr s1 s2 now (now + period) ->
-    O <> 0 ->
-    (now + period > Δ) ->
-    exists tr,
-      In tr (m_ledger s2) /\
-      tr_from tr = I /\
-      tr_to tr = O /\
-      tr_amount tr = sc * 11.
-Proof.
-
-
-Lemma zcb_step_I_to_O :
-  forall s1 s2 ctr_id dsc_id now period I O sc ctr,
-    is_executed ctr s1 s2 O ->
-    consistent_state s1 ->
-    ctr = finctr ctr_id dsc_id (zcb_desc now period) I O O sc ->
-    
-    exists tr,
-      In tr (m_ledger s2) /\
-      tr_ctr_id tr = ctr_id /\
-      tr_from tr = I /\
-      tr_to tr = O /\
-      tr_amount tr = sc * 11.
-Proof.
-
-
-Lemma zcb_step_I_to_O :
-  forall s1 s2 ctr_id dsc_id now period I O sc ctr,
-    step s1 s2 ->
-    consistent_state s1 ->
-    ctr = finctr ctr_id dsc_id (zcb_desc now period) I O O sc ->
-    In ctr (m_contracts s1) ->
-    In (Executed ctr_id) (m_events s2) ->
-    O <> 0 ->
-    (m_global_time s2) > now + period - Δ ->
-    exists tr,
-      In tr (m_ledger s2) /\
-      tr_ctr_id tr = ctr_id /\
-      tr_from tr = I /\
-      tr_to tr = O /\
-      tr_amount tr = sc * 11.
-Proof.
-  intros.
-  induction H.
-  - subst s2. find_contradiction H2.
-    destruct H3 as [H3 | H3]; try inversion H3; try contradiction.
-  - ctr_case_analysis ctr ctr0.
-    subst ctr s2. simpl in *.
-    destruct H3 as [H3 | H3]; try contradiction. clear H3.
-    + unfold exec_ctr_in_state_with_owner in H11.
-      simpl in H11. inversion H11. clear H11.
-      case_analysis H3.
+  - insert_consistent s Ss.
+    insert_consistent s' Ss.
+    induction St; subst s'.
+    + inversion_event Ev. find_contradiction M.
+    + ctr_case_analysis ctr ctr0.
+      execute_own ctr H12.
       case_analysis H12.
-      * simpl. eexists. split.
-        ** left. eauto.
-        ** repeat split; trivial. simpl. resolve_owner H6.
-      * apply ltb_sound_false in H3.
-        apply ltb_sound_false in H1.
-        contradict H3. omega.
-  - ctr_case_analysis ctr ctr0. subst ctr s2.
-    unfold zcb_desc in H8. inversion H8.
-  - ctr_case_analysis ctr ctr0. subst ctr s2.
-    unfold zcb_desc in H8. inversion H8.
-  - ctr_case_analysis ctr ctr0. subst ctr s2.
-    simpl in H3.
-    destruct H3 as [H3 | H3]; try inversion H3.
-    find_contradiction H2.
-  - subst. simpl in *. find_contradiction H2.
+      case_analysis H15.
+      * rewrite <- T0 in *.
+        apply ltb_sound_true in H12.
+        apply ltb_sound_false in H0.
+        contradict H0. unfold Δ. omega.
+      * simpl in *. 
+        rewrite H0, H12 in Exec.
+        inversion Exec. subst res.
+        simpl in M0, J. destruct M0 as [M0 | M0]; try contradiction.
+        eapply O_joins_generated_too_late_inner; eauto.
+    + not_or ctr ctr0 H9.
+    + not_or ctr ctr0 H9.
+    + ctr_case_analysis ctr ctr0. inversion_event Ev. find_contradiction M.
+    + find_contradiction M.
 Qed.
 
-
-Lemma zcb_steps_I_to_O :
-  forall s1 s2 ctr_id dsc_id now period I O sc ctr,
-    steps s1 s2 ->
-    consistent_state s1 ->
-    ctr = finctr ctr_id dsc_id (zcb_desc now period) I O O sc ->
-    In ctr (m_contracts s1) ->
-    In (Executed ctr_id) (m_events s2) ->
-    O <> 0 ->
-    (m_global_time s2) > now + period - Δ ->
-    exists s s', steps s1 s /\ step s s' /\ steps s' s2 /\ In 
-    exists tr,
-      In tr (m_ledger s2) /\
-      tr_ctr_id tr = ctr_id /\
-      tr_from tr = I /\
-      tr_to tr = O /\
-      tr_amount tr = sc * 11.
-Proof.
-
-
-Lemma zcb_step_I_to_O' :
-  forall s1 s2 ctr_id dsc_id now period I O sc ctr,
-    step s1 s2 ->
-    consistent_state s1 ->
-    ctr = finctr ctr_id dsc_id (zcb_desc now period) I O O sc ->
-    In ctr (m_contracts s1) ->
-    In (Executed ctr_id) (m_events s2) ->
-    O <> 0 ->
-    (m_global_time s1) <= now + period - Δ ->
-    exists ctr,
-      In ctr (m_contracts s2) /\
-      ctr_primitive ctr = (At (now + period) (Scale 11 (One USD))) /\
-      ctr_issuer ctr = I /\
-      ctr_proposed_owner ctr = O /\
-      ctr_scale ctr = sc.
-Proof.
-  intros.
-  induction H.
-  - subst s2. find_contradiction H2.
-    destruct H3 as [H3 | H3]; try inversion H3; try contradiction.
-  - ctr_case_analysis ctr ctr0.
-    subst ctr s2. simpl in *.
-    destruct H3 as [H3 | H3]; try contradiction.
-    + unfold exec_ctr_in_state_with_owner in *.
-      simpl in H11. inversion H11.
-      case_analysis H11.
-      case_analysis H14.
-      * apply ltb_sound_true in H12.
-        apply ltb_sound_false in H1.
-        omega.
-      * eexists. split; simpl.
-        ** rewrite in_app_iff. right. simpl. left. eauto.
-        ** repeat split; trivial. resolve_owner H6.
-  - ctr_case_analysis ctr ctr0. subst ctr s2.
-    unfold zcb_desc in H8. inversion H8.
-  - ctr_case_analysis ctr ctr0. subst ctr s2.
-    unfold zcb_desc in H8. inversion H8.
-  - ctr_case_analysis ctr ctr0. subst ctr s2.
-    simpl in H3.
-    destruct H3 as [H3 | H3]; try inversion H3.
-    find_contradiction H2.
-  - subst. simpl in *. find_contradiction H2.
-Qed.
-
-
-
-
-
-
-
-
-(*
-
-
-
-
-WHOAAAA
-
- *)
-
-
-
-Lemma zcb_step_I_to_O'' :
-  forall s1 s2 ctr_id dsc_id period I O sc ctr,
-    step s1 s2 ->
-    consistent_state s1 ->
-    ctr = finctr ctr_id dsc_id (zcb_desc (m_global_time s1) period) I O O sc ->
-    In ctr (m_contracts s1) ->
-    In (Executed ctr_id) (m_events s2) ->
-    O <> 0 ->
-    (m_global_time s2) > (m_global_time s1) + period - Δ ->
-    exists tr,
-      In tr (m_ledger s2) /\
-      tr_ctr_id tr = ctr_id /\
-      tr_from tr = I /\
-      tr_to tr = O /\
-      tr_amount tr = sc * 11.
-Proof.
-  intros.
-  induction H.
-  - subst s2. find_contradiction H2.
-    destruct H3 as [H3 | H3]; try inversion H3; try contradiction.
-  - ctr_case_analysis ctr ctr0.
-    subst ctr s2. simpl in *.
-    destruct H3 as [H3 | H3]; try contradiction. clear H3.
-    unfold exec_ctr_in_state_with_owner in H11.
-    simpl in H11. inversion H11. clear H11.
-    case_analysis H3.
-    case_analysis H11.
-    * eexists. split.
-      ** simpl. left. eauto.
-      ** repeat split; trivial. resolve_owner H6.
-    *  apply ltb_sound_false in H1.
-       apply ltb_sound_false in H3.
-       contradict H3. omega.
-  - ctr_case_analysis ctr ctr0. subst ctr s2.
-    unfold zcb_desc in H8. inversion H8.
-  - ctr_case_analysis ctr ctr0. subst ctr s2.
-    unfold zcb_desc in H8. inversion H8.
-  - ctr_case_analysis ctr ctr0. subst ctr s2.
-    simpl in H3.
-    destruct H3 as [H3 | H3]; try inversion H3.
-    find_contradiction H2.
-  - subst. simpl in *. find_contradiction H2.
-Qed.
-
-
-Lemma gt_implies_ge_Sn :
-  forall n m,
-    n > m -> n >= S m.
-Admitted.
-
-Lemma ge_implies_eq_or_gt:
-  forall n m,
-    n >= m -> n = m \/ n > m.
-Admitted.
-
-
-
-Lemma helper1 :
-  forall s1 s2 ctr period O,
-    steps s1 s2 ->
-    In ctr (m_contracts s1) ->
-    consistent_state s1 ->
-    In (Executed (ctr_id ctr)) (m_events s2) ->
-    ctr_primitive ctr = zcb_desc (m_global_time s1) period ->
-    O <> 0 ->
-    m_global_time s2 > m_global_time s1 + period -  Δ.
-Proof.
-  intros.
-  induction H.
-  - subst s2. find_contradiction H2.
-  - assert (H' := H). assert (H'' := H).
-    apply steps_preserves_consistent_state in H'; auto.
-    apply steps_effect_over_contract with (ctr := ctr) in H; trivial.
-    destruct H as [H|[H|H]]; trivial.
-    + induction H5; subst s2; simpl.
-      ++ simpl in H2. destruct H2 as [H2 | H2]; try inversion H2.
-         find_contradiction H0.
-      ++ ctr_case_analysis ctr ctr0.
-         simpl in H2. destruct H2 as [H2 | H2]; try contradiction. clear H2.
-         unfold exec_ctr_in_state_with_owner in H11. rewrite H3 in H11.
-         simpl in H11.
-         case_analysis H11.
-         case_analysis H14.
-         ** apply ltb_sound_true in H11. auto.
-         ** apply ltb_sound_false in H11.
-            apply ltb_sound_false in H2.
-         
-
-    + eapply IHsteps in H. admit.
-    + admit.
-Admitted.
-
-
-Lemma zcb_steps_I_to_O'' :
-  forall s1 s2 ctr_id dsc_id period I O sc ctr,
-    steps s1 s2 ->
-    consistent_state s1 ->
-    ctr = finctr ctr_id dsc_id (zcb_desc (m_global_time s1) period) I O O sc ->
-    In ctr (m_contracts s1) ->
-    In (Executed ctr_id) (m_events s2) ->
-    O <> 0 ->
-    period - Δ > 0 ->
-    (m_global_time s2) > (m_global_time s1) + period - Δ ->
-    exists tr,
-      In tr (m_ledger s2) /\
-      tr_ctr_id tr = ctr_id /\
-      tr_from tr = I /\
-      tr_to tr = O /\
-      tr_amount tr = sc * 11.
-Proof.
-  intros.
-  induction H.
-  - subst. find_contradiction H2.
-  - assert (H' := H). assert (H'' := H).
-    apply steps_preserves_consistent_state in H'; auto.
-    apply steps_effect_over_contract with (ctr := ctr) in H; trivial.
-    destruct H as [H|[H|H]]; trivial.
-    + eapply zcb_step_I_to_O; eauto.
-    + rewrite H1 in H. simpl in H.
-      eapply helper1 with (period := period) in H''; eauto.
-      ++ eapply IHsteps in H''; eauto.
-         destruct H'' as [tr [H'' H''']].
-         eexists. split; eauto.
-         eapply step_does_not_remove_transactions; eauto.
-      ++ subst ctr. trivial.
-      ++ subst ctr. trivial.
-    + assert (C := H7). rewrite H1 in H. simpl in H.
-      eapply step_preserves_consistent_state in C; eauto.
-      eapply step_does_not_remove_events in H7.
-      unfold consistent_state in C.
-      destruct C as [_ [_ [_ [_ C]]]].
-      unfold not in C.
-      exfalso. eapply C; eauto.
-      trivial.
-Admitted.
-
-
-
-      assert (HT := H7).
-      assert (N : m_global_time s > m_global_time s1 + period + Δ).
-      {
-        induction H''; intros.
-        - subst s0. find_contradiction H.
-        - induction H8; subst s0.
-          + simpl in *. destruct H as [H | H]; try inversion H.
-            apply IHH'' in H; auto.
-
-
-        }
-      eapply timebound_steps in H; eauto.
-
-      apply gt_implies_ge_Sn in H6.
-      eapply time_passes_one_step_at_a_time in H6; eauto.
-      apply ge_implies_eq_or_gt in H6.
-      destruct H6 as [H6 | H6].
-      ++ rewrite H6 in *.
-
-      eapply zcb_step_I_to_O''; eauto.
-    + subst ctr. simpl in *.
-      apply IHsteps in H.
-      destruct H as [tr [H HT]].
-      exists tr.
-      split; trivial.
-      eapply step_does_not_remove_transactions; eauto.
-    + eapply step_preserves_consistent_state in H'; eauto.
-      eapply step_does_not_remove_events in H5; eauto.
-      destruct H' as [_ [_ [_ [_ T]]]].
-      unfold not in T.
-      exfalso.
-      eapply T. subst ctr.
-      split; eauto.
-Qed.
-
+Print O_joins_generated_too_late.
